evset.v
@@ -1,0 +1,82 @@
+Require Import List.
+Require Import Coq.Arith.EqNat.
+
+Definition IdEv : Set := nat.
+
+Definition Input : Set := bool.
+Parameter Output : Set.
+(*
+Definition Output : Set := nat.
+Parameter Pred : nat -> Input.
+Parameter Act : nat -> Output.
+*)
+
+Definition Pred : Set := nat -> Input.
+Definition Act : Set := nat -> Output.
+
+Inductive Event : Set :=
+  Eps : Event
+| EIn : IdEv -> Pred -> Event
+| EOut : IdEv -> Act -> Event.
+
+Definition EvSet := list Event.
+
+Definition empty_set : EvSet := nil.
+
+
+
+(* cual me conviene mas? dejo los dos? *)
+Inductive Beq_event : Event -> Event -> Prop :=
+  beq_eps : Beq_event Eps Eps
+| beq_in : forall (i:IdEv)(p1 p2:Pred), Beq_event (EIn i p1)(EIn i p2)
+| beq_out : forall (i:IdEv)(a1 a2:Act), Beq_event (EOut i a1)(EOut i a2).
+
+Definition beq_event (e1 e2: Event) : bool := match e1, e2 with
+  Eps, Eps => true
+| EIn i1 p1 , EIn i2 p2 => beq_nat i1 i2
+| EOut i1 a1 , EOut i2 a2 => beq_nat i1 i2
+| _ , _ => false end.
+
+Notation "a == b" := (Beq_event a b) (at level 70, no associativity).
+
+Theorem eq_event_true : forall (e1 e2:Event), beq_event e1 e2 = true -> Beq_event e1 e2.
+Proof.
+  intros e1 e2 H.
+  induction e1;induction e2.
+  constructor.
+  simpl in H.
+  inversion H.
+  simpl in H.
+  inversion H.
+  simpl in H.
+  inversion H.
+  simpl in H.
+  rewrite (beq_nat_true i i0).
+  constructor.
+  assumption.
+  inversion H.
+  inversion H.
+  simpl in H.
+  inversion H.
+  rewrite (beq_nat_true i i0).
+  constructor.
+  assumption.
+Qed.
+
+Definition Aeq_dec: forall a b:Event, {a == b} + {a <> b}.
+
+
+Fixpoint set_add (e:Event) (x:EvSet) : EvSet :=
+    match x with
+    | nil => cons e nil
+    | cons e1 x1 => if beq_event e e1 then cons e1 x1 else cons e1 (set_add e x1)
+    end.
+
+Inductive isMember: Event -> EvSet -> Prop :=
+  sing: forall (e f:Event)(s:EvSet), Beq_event e f -> isMember e (cons f s)
+| cons: forall (e f:Event)(s:EvSet), isMember e s -> isMember e (f :: s).
+
+Fixpoint isElem (e:Event)(s:EvSet) : bool := match s with
+  nil => false
+| x :: xs => if beq_event e x then true else isElem e xs
+end.
